src/ChurchRosser.lean
@@ -1,0 +1,57 @@
+import Cslib.Languages.LambdaCalculus.LocallyNameless.Untyped.FullBeta
+import Cslib.Languages.LambdaCalculus.LocallyNameless.Untyped.FullBetaConfluence
+
+
+namespace Cslib
+namespace LambdaCalculus.LocallyNameless.Untyped.Term
+
+open Term
+
+universe u
+variable {Var : Type u} [HasFresh Var] [DecidableEq Var]
+
+
+def multiBeta (M N : Term Var) : Prop := M ↠βᶠ N
+
+#check Relation.ChurchRosser -- Cslib
+-- #check Relation.church_rosser -- Mathlib
+
+theorem ChurchRosserMultiBeta : Relation.ChurchRosser (@multiBeta Var) := by
+  unfold multiBeta
+  intro x y h_equiv
+
+  have h_equiv_base : Relation.EqvGen FullBeta x y := by
+    induction h_equiv
+    case refl => apply Relation.EqvGen.refl
+    case symm ih => apply Relation.EqvGen.symm; assumption
+    case rel h =>
+      induction h
+      case refl a b => apply Relation.EqvGen.refl
+      case tail a b c d e f g h =>
+        apply Relation.EqvGen.trans _ d
+        · assumption
+        · apply Relation.EqvGen.rel
+          assumption
+    case trans a b c d e f g h i =>
+      apply Relation.EqvGen.trans _ d
+      · assumption
+      · assumption
+
+  have h_cr := Relation.Confluent.toChurchRosser confluence_beta h_equiv_base
+
+  obtain ⟨z, hxz, hyz⟩ := h_cr
+  use z
+  constructor
+  · apply Relation.ReflTransGen.single
+    exact hxz
+  · apply Relation.ReflTransGen.single
+    exact hyz
+
+theorem ChurchRosserMultiBeta':
+    ∀ (M N : Term Var), multiBeta M N → ∃ P : Term Var, multiBeta M P ∧ multiBeta N P := by
+  intro M N hMN
+  refine ⟨N, hMN, ?_⟩
+  exact Relation.ReflTransGen.refl
+
+end LambdaCalculus.LocallyNameless.Untyped.Term
+end Cslib
