src/LambdaTerms.lean
@@ -1,0 +1,17 @@
+import Cslib.Languages.LambdaCalculus.LocallyNameless.Untyped.FullBeta
+
+namespace Cslib
+namespace LambdaCalculus.LocallyNameless.Untyped.Term
+
+open Term
+
+namespace LambdaTerms
+
+universe u
+variable {Var : Type u}
+
+def K     : Term Var := abs (abs $ bvar 1) -- λxy.x
+def Kstar : Term Var := abs (abs $ bvar 0) -- λxy.y
+def id    : Term Var := abs (bvar 0)       -- λx.x
+
+end LambdaTerms
