src/LambdaTheory/Basic.lean
@@ -1,0 +1,65 @@
+import Cslib.Languages.LambdaCalculus.LocallyNameless.Untyped.FullBeta
+import src.BetaEquiv
+
+open Cslib
+open LambdaCalculus.LocallyNameless.Untyped
+
+open Term
+
+namespace LambdaTheory
+
+universe u
+variable {Var : Type u}
+
+-- Herman Geuvers (https://www.cs.ru.nl/~herman/onderwijs/semantics2025/model_untyped_lambda.pdf)
+-- A λ-theory is closed under the following six rules
+class LambdaTheory (rel: Term Var → Term Var → Prop) where
+  beta (M N : Term Var) : FullBeta M N → rel M N
+  app (M N P Q : Term Var) : rel M N → rel P Q → rel (Term.app M P) (Term.app N Q)
+-- | xi (M N) : LambdaRelated M N → Term.abs
+  refl (M : Term Var) : rel M M
+  trans (M N P : Term Var) : rel M N → rel N P → rel M P
+  sym (M N : Term Var): rel M N → rel N M
+
+
+variable {r : Term Var → Term Var → Prop} [LambdaTheory r]
+
+@[simp, grind .]
+lemma ThEq_of_BetaEquiv {M N : Term Var} {r : Term Var → Term Var → Prop} [LambdaTheory r] (h : M ≡β N) : r M N := by
+  induction h with
+  | rel _ _ h => apply LambdaTheory.beta; assumption
+  | refl => apply LambdaTheory.refl
+  | symm M N h ih => apply LambdaTheory.sym; assumption
+  | trans M N P h₁ h₂ ih₁ ih₂ =>
+    apply LambdaTheory.trans M N P
+    · assumption
+    · assumption
+
+-- This way we can use calc blocks when reasoning over equality in a theory
+instance : Trans r r r where
+  trans {M N P} h1 h2 := LambdaTheory.trans M N P h1 h2
+
+@[refl]
+lemma refl' (M : Term Var) : r M M :=
+  LambdaTheory.refl M
+
+@[symm]
+lemma sym' {M N : Term Var} (h : r M N) : r N M :=
+  LambdaTheory.sym M N h
+
+lemma app_left {M N : Term Var} (P : Term Var) (h : r M N) :
+  r (Term.app M P) (Term.app N P) :=
+  LambdaTheory.app M N P P h (LambdaTheory.refl P)
+
+lemma app_right (M : Term Var) {P Q : Term Var} (h : r P Q) :
+  r (Term.app M P) (Term.app M Q) :=
+  LambdaTheory.app M M P Q (LambdaTheory.refl M) h
+
+lemma app_left₂ {M N : Term Var} (P Q : Term Var) (h : r M N) :
+  r (Term.app (Term.app M P) Q) (Term.app (Term.app N P) Q) :=
+  app_left Q (app_left P h)
+
+
+def inconsistent (r : Term Var → Term Var → Prop) [LambdaTheory r] : Prop := ∀ M N : Term Var, M.LC → N.LC → r M N
+
+end LambdaTheory
