src/LambdaTheory/KeqKstar.lean
@@ -1,0 +1,159 @@
+import src.LambdaTheory.Basic
+import src.LambdaTerms
+import src.BetaEquiv
+import Cslib.Languages.LambdaCalculus.LocallyNameless.Untyped.FullBeta
+
+open Cslib
+open LambdaCalculus.LocallyNameless.Untyped
+open Term
+
+open LambdaTerms
+open LambdaTheory
+
+universe u
+variable {Var : Type u} [HasFresh Var] [DecidableEq Var]
+
+inductive ThKeqKstar : Term Var → Term Var → Prop
+| beta (M N) : FullBeta M N → ThKeqKstar M N
+| app (M N P Q) : ThKeqKstar M N → ThKeqKstar P Q → ThKeqKstar (Term.app M P) (Term.app N Q)
+-- | xi (M N) : LambdaRelated M N → Term.abs
+| refl (M) : ThKeqKstar M M
+| trans (M N P) : ThKeqKstar M N → ThKeqKstar N P → ThKeqKstar M P
+| sym (M N): ThKeqKstar M N → ThKeqKstar N M
+| new : ThKeqKstar K Kstar
+
+instance instKeqKstar : @LambdaTheory Var ThKeqKstar :=
+    ⟨ThKeqKstar.beta, ThKeqKstar.app, ThKeqKstar.refl, ThKeqKstar.trans, ThKeqKstar.sym⟩
+
+
+lemma Kstar_LC {Var : Type u} : (@Kstar Var).LC := by
+  unfold Kstar
+  apply LC.abs
+  intro x _
+  apply LC.abs
+  intro y _
+  simp
+  apply LC.fvar
+  · exact Finset.empty
+  exact Finset.empty
+
+lemma reduceKstar {Var : Type u} (M : Term Var) (hM : M.LC) : (@app Var Kstar M) →βᶠ (abs $ bvar 0) := by
+  unfold Kstar
+
+  constructor
+  constructor
+  · apply LC.abs
+    intro x _
+    apply LC.abs
+    intro y _
+    simp
+    apply LC.fvar
+    · exact Finset.empty
+    · exact Finset.empty
+  · exact hM
+
+lemma reduceKstar2 {Var : Type u} (M N : Term Var) (hM : M.LC) (hN : N.LC) : (@app Var (@app Var Kstar M) N) ↠βᶠ N := by
+  -- unfold Kstar
+  apply Relation.ReflTransGen.tail (b := app (abs $ bvar 0) N)
+  apply Relation.ReflTransGen.single
+  apply Xi.appR
+  · assumption
+  · apply reduceKstar
+    · assumption
+  · constructor
+    constructor
+    apply LC.abs
+    grind
+    exact Finset.empty
+    assumption
+
+lemma K_LC {Var : Type u} : (@K Var).LC := by
+  unfold K
+  apply LC.abs
+  intro x _
+  apply LC.abs
+  intro y _
+  apply LC.fvar
+  · exact Finset.empty
+  exact Finset.empty
+
+
+lemma KstarMN_eq_N (M N : Term Var) (hM : M.LC) (hN : N.LC) : app (app Kstar M) N ≡β N := by
+  apply betaEquiv_of_multiBeta
+  · constructor
+    swap; assumption
+    constructor
+    swap; assumption
+    exact Kstar_LC
+  · assumption
+  · apply reduceKstar2
+    · assumption
+    · assumption
+
+lemma reduceK {Var : Type u} (M N : Term Var) (hM : M.LC) (hN : N.LC) : (app (app K M) N) ↠βᶠ M := by
+  unfold K
+  apply Relation.ReflTransGen.tail (b := app (abs $ bvar 1) N)
+  apply Relation.ReflTransGen.single
+  apply Xi.appR
+  · assumption
+  · sorry
+  sorry
+
+-- instance : CoeFun (Term Var) (fun _ => Term Var → Term Var) where
+--   coe M N := Term.app M N
+
+@[simp]
+lemma K_MN_eq_M (M N : Term Var) (hM : M.LC) (hN : N.LC) : app (app K M) N ≡β M := by
+  apply betaEquiv_of_multiBeta
+  · apply LC.app
+    · apply LC.app
+      · exact K_LC
+      · assumption
+    · assumption
+  · assumption
+  · apply reduceK
+    · assumption
+    · assumption
+
+local notation:50 M " =K= " N => ThKeqKstar M N
+
+-- We prove that adding K = Kstar results in an inconsistent λ-theory
+lemma K_eq_Kstart_inconsistent {Var : Type u} [DecidableEq Var] [HasFresh Var] : @inconsistent Var ThKeqKstar instKeqKstar := by
+  intro M N hM hN
+
+  #check Var
+
+  have h₁: M =K= @app Var (@app Var K M) N := by
+    -- apply @ThEq_of_BetaEquiv Var M ((K.app M).app N) ThKeqKstar
+    apply ThEq_of_BetaEquiv
+    -- have t : (M ≡β (K.app M).app N) → (K.app M).app N =K= M := sorry
+    -- have : (M ≡β (K.app M).app N) := sorry
+    -- have t : (@BetaEquiv Var M (@app Var (@app Var K M) N)) → (@ThKeqKstar Var (@app Var (@app Var K M) N) M) := sorry
+    -- have : @ThKeqKstar Var (@app Var (@app Var K M) N) M := sorry
+    symm
+    -- apply t
+    -- exact this
+    -- symm
+    apply K_MN_eq_M
+    assumption
+    assumption
+
+  have h₂: (K.app M).app N =K= (Kstar.app M).app N := by
+    -- simp
+    apply app_left₂
+    apply ThKeqKstar.new
+  have h₃: (Kstar.app M).app N =K= N := by
+    apply ThEq_of_BetaEquiv
+    apply KstarMN_eq_N
+    assumption
+    assumption
+-- M = K M N = Kstar M N = N
+  calc M =K= (K.app M).app N := h₁
+       _ =K= (Kstar.app M).app N := h₂
+       _ =K= N := h₃
+
+
+  -- calc
+  --   M =K= K M N := by simp; apply ThEq_of_BetaEquiv; symm; apply K_MN_eq_M; assumption; assumption
+  --   _ =K= Kstar M N := by simp; apply app_left₂; apply ThKeqKstar.new
+  --   _ =K= N := by simp; apply ThEq_of_BetaEquiv; apply KstarMN_eq_N; assumption; assumption
